Release lock invariants lecture source

go/concurrent/examples.go
@@ -1,0 +1,52 @@
+package concurrent
+
+import "sync"
+
+func SetX(x *uint64) {
+	*x = 1
+}
+
+func NoGo() {
+	var x uint64
+	SetX(&x)
+}
+
+func FirstGo() {
+	var x uint64
+	go func() {
+		SetX(&x)
+	}()
+}
+
+func FirstLock() uint64 {
+	var x uint64
+	m := new(sync.Mutex)
+	go func() {
+		m.Lock()
+		x = 1
+		m.Unlock()
+	}()
+	m.Lock()
+	y := x
+	m.Unlock()
+	return y
+}
+
+func LockedCounter() uint64 {
+	counter := new(uint64)
+	m := new(sync.Mutex)
+	go func() {
+		m.Lock()
+		*counter = *counter + 2
+		m.Unlock()
+	}()
+	go func() {
+		m.Lock()
+		*counter = *counter + 2
+		m.Unlock()
+	}()
+	m.Lock()
+	y := *counter
+	m.Unlock()
+	return y
+}
